PropositionalLogic/Complete/Canonical_Kripke.v
@@ -4,18 +4,21 @@ Require Import Coq.Logic.Classical_Pred_Type.
 Require Import Logic.lib.Bijection.
 Require Import Logic.lib.Countable.
 Require Import Logic.GeneralLogic.Base.
-Require Import Logic.GeneralLogic.HenkinCompleteness.
 Require Import Logic.GeneralLogic.KripkeModel.
+Require Import Logic.GeneralLogic.ProofTheory.BasicSequentCalculus.
+Require Import Logic.GeneralLogic.Semantics.Kripke.
+Require Import Logic.GeneralLogic.Complete.ContextProperty.
+Require Import Logic.GeneralLogic.Complete.ContextProperty_Kripke.
 Require Import Logic.MinimunLogic.Syntax.
-Require Import Logic.PropositionalLogic.Syntax.
-Require Import Logic.MinimunLogic.ProofTheory.Normal.
 Require Import Logic.MinimunLogic.ProofTheory.Minimun.
+Require Import Logic.MinimunLogic.Semantics.Kripke.
+Require Import Logic.MinimunLogic.Complete.ContextProperty_Kripke.
+Require Import Logic.PropositionalLogic.Syntax.
 Require Import Logic.PropositionalLogic.ProofTheory.Intuitionistic.
 Require Import Logic.PropositionalLogic.ProofTheory.DeMorgan.
 Require Import Logic.PropositionalLogic.ProofTheory.GodelDummett.
 Require Import Logic.PropositionalLogic.ProofTheory.Classical.
 Require Import Logic.PropositionalLogic.Semantics.Kripke.
-Require Import Logic.MinimunLogic.Complete.ContextProperty_Intuitionistic.
 Require Import Logic.PropositionalLogic.Complete.ContextProperty_Kripke.
 
 Local Open Scope logic_base.
@@ -28,17 +31,18 @@ Import KripkeModelNotation_Intuitionistic.
 Section Canonical.
 
 Context {L: Language}
-        {nL: NormalLanguage L}
+        {minL: MinimunLanguage L}
         {pL: PropositionalLanguage L}
         {Gamma: ProofTheory L}
-        {nGamma: NormalProofTheory L Gamma}
-        {mpGamma: MinimunPropositionalLogic L Gamma}
-        {ipGamma: IntuitionisticPropositionalLogic L Gamma}
+        {bSC: BasicSequentCalculus L Gamma}
+        {minSC: MinimunSequentCalculus L Gamma}
+        {ipSC: IntuitionisticPropositionalSequentCalculus L Gamma}
         {MD: Model}
         {kMD: KripkeModel MD}
         {M: Kmodel}
         {R: Relation (Kworlds M)}
         {SM: Semantics L MD}
+        {kminSM: KripkeMinimunSemantics L MD M SM}
         {kpSM: KripkePropositionalSemantics L MD M SM}.
 
 Context (P: context -> Prop)
@@ -46,43 +50,11 @@ Context (P: context -> Prop)
 
 Hypothesis H_R: forall m n Phi Psi, rel m Phi -> rel n Psi -> (m <= n <-> Included _ (proj1_sig Phi) (proj1_sig Psi)).
 
-Lemma denote_monotonic (x: expr):
-  (forall m Phi, rel m Phi -> (KRIPKE: M, m |= x <-> proj1_sig Phi x)) ->
-  upwards_closed_Kdenote (Kdenotation M x).
-Proof.
-  intros.
-  hnf; intros.
-  change (KRIPKE: M, m |= x).
-  change (KRIPKE: M, n |= x) in H1.
-  destruct (im_bij _ _ rel n) as [Phi ?].
-  destruct (im_bij _ _ rel m) as [Psi ?].
-  erewrite H in H1 |- * by eauto.
-  eapply H_R in H0; eauto.
-  apply H0; auto.
-Qed.
-
-Instance po_R: PreOrder (@KI.Krelation _ R).
-Proof.
-  constructor.
-  + hnf; intros m.
-    destruct (im_bij _ _ rel m) as [Phi ?].
-    apply (H_R _ _ _ _ H H).
-    hnf; intros; auto.
-  + hnf; intros m1 m2 m3.
-    destruct (im_bij _ _ rel m1) as [Phi1 ?].
-    destruct (im_bij _ _ rel m2) as [Phi2 ?].
-    destruct (im_bij _ _ rel m3) as [Phi3 ?].
-    rewrite (H_R _ _ _ _ H H0).
-    rewrite (H_R _ _ _ _ H0 H1).
-    rewrite (H_R _ _ _ _ H H1).
-    clear; unfold Included, Ensembles.In; firstorder.
-Qed.
-
 Lemma classical_canonical_ident
-      {cpGamma: ClassicalPropositionalLogic L Gamma}
-      (DER: at_least_derivable_closed P)
-      (ORP: at_least_orp_witnessed P)
-      (CONSI: at_least_consistent P):
+      {cpSC: ClassicalPropositionalSequentCalculus L Gamma}
+      (AL_DC: at_least derivable_closed P)
+      (AL_OW: at_least orp_witnessed P)
+      (AL_CONSI: at_least consistent P):
   IdentityKripkeIntuitionisticModel (Kworlds M).
 Proof.
   constructor.
@@ -97,16 +69,16 @@ Proof.
   intros; split; [apply H; auto |].
   intros.
   pose proof derivable_excluded_middle (proj1_sig Phi) x.
-  rewrite <- derivable_closed_element_derivable in H1 by (apply DER, (proj2_sig Phi)).
-  apply ORP in H1; [| apply (proj2_sig Phi)].
+  rewrite <- derivable_closed_element_derivable in H1 by (apply AL_DC, (proj2_sig Phi)).
+  apply AL_OW in H1; [| apply (proj2_sig Phi)].
   destruct H1; auto.
   exfalso.
   apply H in H1; unfold Ensembles.In in H1.
-  rewrite derivable_closed_element_derivable in H0, H1 by (apply DER, (proj2_sig Psi)).
+  rewrite derivable_closed_element_derivable in H0, H1 by (apply AL_DC, (proj2_sig Psi)).
   pose proof deduction_modus_ponens _ _ _ H0 H1.
   revert H2; change (~ proj1_sig Psi |-- FF).
   rewrite <- consistent_spec.
-  apply CONSI, (proj2_sig Psi).
+  apply AL_CONSI, (proj2_sig Psi).
 Qed.
 
 Lemma GodelDummett_canonical_no_branch
